\chapter{Appendix}

\section{Proof of Lemma~\ref{lemma:mis-eav-from-eav}} \label{sec:mis-eav-from-eav-proof}

\begin{proof}[of Lemma~\ref{lemma:mis-eav-from-eav}] Note that since the message space is finite, the time to encrypt a message is bounded. As outlined before Lemma~\ref{lemma:mis-eav-from-eav}, the lemma follows from a simple hybrid argument. Let $q$ a function in $\kappa$, let $\kappa$ arbitrary and let $\adv$ an arbitrary MIS-EAV adversary running in time $\tilde{t}(\kappa)$ and making at most $q(\kappa)$ queries. Define the sequence of hybrid games $H_0, \ldots, H_q$ where in the game $H_i$ the first $i$ encryptions given to the adversary encrypt $m_1$ and all remaining encryptions encrypt $m_0$. We will write
	\[
		\pr{0 \from \adv \mid H_i}
	\]
	for the probability of $\adv$ outputting $0$ when playing the hybrid game $H_i$.

	Let $i \in [q]$. Construct an EAV adversary $\adv'$ that behaves as follows:
	\begin{enumerate}[1.]
		\item $\adv'$ runs $\adv$ and gets $q, m_0, m_1$.
		\item $\adv'$ outputs the messages $m_0, m_1$ and gets a ciphertext $c$ from the challenger.
		\item $\adv'$ gives the ciphertexts $c_1, \ldots, c_q$ to $\adv$ where
		      \[
			      c_j = \begin{cases}
				      \Pi.\enc_{k_j}(m_1) & i < j \\
				      c                   & i = j \\
				      \Pi.\enc_{k_j}(m_0) & i > j
			      \end{cases}
		      \]
		      and $k_j \from \Pi.\gen(1^\kappa) \; \forall j$.
		\item $\adv'$ outputs whatever bit $\adv$ outputs.
	\end{enumerate}
	Now consider the value of the bit $b$ sampled in $\game{\Pi}{\kappa}{EAV}(\adv')$. If $b = 0$, then the first $i - 1$ ciphertexts that $\adv$ received were encryptions of $m_1$ and the remaining ciphertexts were encryptions of $m_0$, where all encryptions were under keys sampled independently with $\Pi.\gen$. Thus, from the view of $\adv$ everything followed the same distribution as in the game $H_{i - 1}$ and
	\[
		\pr{0 \from \adv' \mid b = 0} = \pr{0 \from \adv \mid H_{i - 1}}.
	\]
	Analogously, in the case $b = 1$ the first $i$ ciphertexts received by $\adv$ were encryptions of $m_1$ and the rest encryptions of $m_0$, so
	\[
		\pr{0 \from \adv' \mid b = 1} = \pr{0 \from \adv \mid H_{i}}.
	\]
	Then
	\begin{align} \label{eq:eav-to-mis-eav-hybrid-distinguisher}
		\begin{split}
			\begin{split}
				\pr{0 \from \adv \mid H_{i - 1}} - & \pr{0 \from \adv \mid H_{i}} \\
				& = \pr{0 \from \adv' \mid b = 0} - \pr{0 \from \adv' \mid b = 1}
			\end{split} \\
			& \stackrel{\mathclap{\eqref{eq:advantage-equality}}}{=} \advantage{\Pi}{\kappa}{EAV}(\adv')                                         \\
			& \le \epsilon
		\end{split}
	\end{align}
	by $(t, \epsilon)$-EAV security of $\Pi$ since $\adv'$ runs in time $\tilde{t} + \mathcal{O}(q \cdot (t_{\gen} + t_{\enc})) = t$.

	Now let $b$ be the bit sampled in the MIS-EAV game. Notice that
	\[
		\pr{0 \from \adv \mid b = 0} = \pr{0 \from \adv \mid H_0}
	\]
	and
	\[
		\pr{0 \from \adv \mid b = 1} = \pr{0 \from \adv \mid H_q}.
	\]
	Then
	\begin{align*}
		\advantage{\Pi}{\kappa}{MIS-EAV}(\adv) & \stackrel{\mathclap{\eqref{eq:advantage-equality}}}{=} \; \pr{0 \from \adv \mid b = 0} - \pr{0 \from \adv \mid b = 1} \\
		                                       & = \pr{0 \from \adv \mid H_0} - \pr{0 \from \adv \mid H_q}                                                             \\
		                                       & = \sum_{i = 1}^{q} \pr{0 \from \adv \mid H_{i - 1}} - \pr{0 \from \adv \mid H_i}                                      \\
		                                       & \stackrel{\mathclap{\eqref{eq:eav-to-mis-eav-hybrid-distinguisher}}}{\le} q \cdot \epsilon.
	\end{align*}
\end{proof}
